examples/formal-languages/context-free/simpleSexpPEGScript.sml
@@ -4,173 +4,191 @@ open simpleSexpTheory pegTheory pegLib
 
 val _ = new_theory "simpleSexpPEG";
 
-val tokeq_def = Define`tokeq t = tok ((=) t) (K (SX_SYM [t]))`
-val grabWS_def = Define`
+Definition tokeq_def: tokeq t = tok ((=) t) (K (SX_SYM [t]))
+End
+Definition grabWS_def:
   grabWS s = rpt (tok isSpace (K arb_sexp)) (K arb_sexp) ~> s
-`;
+End
 
-val peg0_tokeq = store_thm(
-  "peg0_tokeq[simp]",
-  ``peg0 G (tokeq t) = F``,
-  simp[tokeq_def])
+Theorem peg0_tokeq[simp]: peg0 G (tokeq t) = F
+Proof simp[tokeq_def]
+QED
 
-val pnt_def = Define`pnt ntsym = nt (mkNT ntsym) I`
+Definition pnt_def: pnt ntsym = nt (mkNT ntsym) I
+End
 
-val replace_nil_def= Define`
+Definition replace_nil_def:
   (replace_nil (SX_SYM s) z = if s = "nil" then z else SX_SYM s) ∧
   (replace_nil (SX_CONS x y) z = SX_CONS x (replace_nil y z)) ∧
   (replace_nil x y = x)
-`;
+End
 
 (* have to use these versions of choicel and pegf below because the
    versions from pegTheory use ARB in their definitions.
    Logically, the ARBs are harmless, but they completely mess with the
    CakeML translator.
 *)
-val choicel_def = Define`
+Definition choicel_def:
   choicel [] = not (empty arb_sexp) arb_sexp ∧
   choicel (h::t) = choice h (choicel t) (λs. case s of INL x => x | INR y => y)
-`;
+End
 
-val pegf_def = Define`pegf sym f = seq sym (empty arb_sexp) (λl1 l2. f l1)`;
+Definition pegf_def:
+  pegf sym f = seq sym (empty arb_sexp) (λl1 l2. f l1)
+End
 
-val peg_eval_choicel_NIL = store_thm(
-  "peg_eval_choicel_NIL[simp]",
-  ``peg_eval G (i0, choicel []) x = (x = NONE)``,
-  simp[choicel_def, Once peg_eval_cases]);
+Theorem peg_eval_choicel_NIL[simp]:
+  peg_eval G (i0, choicel []) x <=> x = Failure (sloc i0) G.notFAIL
+Proof simp[choicel_def, Once peg_eval_cases]
+QED
 
-val peg_eval_choicel_CONS = store_thm(
-  "peg_eval_choicel_CONS",
-  ``∀x. peg_eval G (i0, choicel (h::t)) x ⇔
-          peg_eval G (i0, h) x ∧ x <> NONE ∨
-          peg_eval G (i0,h) NONE ∧ peg_eval G (i0, choicel t) x``,
+Theorem peg_eval_choicel_CONS:
+  ∀x. peg_eval G (i0, choicel (h::t)) x ⇔
+      peg_eval G (i0, h) x ∧ isSuccess x ∨
+      ∃r1 r2.
+        peg_eval G (i0,h) r1 ∧ isFailure r1 ∧ peg_eval G (i0, choicel t) r2 ∧
+        x = if isFailure r2 then rmax r1 r2 else r2
+Proof
   simp[choicel_def, SimpLHS, Once peg_eval_cases] >>
-  simp[pairTheory.FORALL_PROD, optionTheory.FORALL_OPTION]);
+  simp[pairTheory.FORALL_PROD, FORALL_result, EXISTS_result,
+       AllCaseEqs()] >> metis_tac[]
+QED
 
-val peg0_choicel = store_thm(
-  "peg0_choicel[simp]",
-  ``(peg0 G (choicel []) = F) ∧
-    (peg0 G (choicel (h::t)) ⇔ peg0 G h ∨ pegfail G h ∧ peg0 G (choicel t))``,
-  simp[choicel_def])
+Theorem peg0_choicel[simp]:
+  (peg0 G (choicel []) = F) ∧
+  (peg0 G (choicel (h::t)) ⇔ peg0 G h ∨ pegfail G h ∧ peg0 G (choicel t))
+Proof simp[choicel_def]
+QED
 
-val peg0_pegf = store_thm(
-  "peg0_pegf[simp]",
-  ``peg0 G (pegf s f) = peg0 G s``,
-  simp[pegf_def])
+Theorem peg0_pegf[simp]:
+  peg0 G (pegf s f) = peg0 G s
+Proof simp[pegf_def]
+QED
 
-val sexpPEG_def = zDefine`
-  sexpPEG : (char, sexpNT, sexp) peg = <|
+Definition sexpPEG_def[nocompute]:
+  sexpPEG : (char, sexpNT, sexp, string) peg =
+  <|
     start := pnt sxnt_sexp ;
+    anyEOF := "Unexpected EOF (any)";
+    tokFALSE := "Failed to see expected token";
+    tokEOF := "Failed to see expected token because of EOF";
+    notFAIL := "Failed to fail in a not rule";
     rules :=
     FEMPTY |++
-    [(mkNT sxnt_sexp, pnt sxnt_WSsexp <~ rpt (tok isSpace (K arb_sexp)) (K arb_sexp));
-     (mkNT sxnt_sexp0,
-      choicel [
-        pnt sxnt_sexpnum ;
-        tokeq #"(" ~> pnt sxnt_sexpseq ;
-        tokeq #"\"" ~> pnt sxnt_strcontents <~ tokeq #"\"" ;
-        pegf (tokeq #"'" ~> grabWS (pnt sxnt_sexp0))
-             (λs. ⟪ SX_SYM "quote"; s⟫) ;
-        pnt sxnt_sexpsym
-      ]);
-     (mkNT sxnt_sexpseq,
-      choicel [
-        pegf (grabWS (tokeq #")")) (K (SX_SYM "nil"));
-        seq (grabWS (pnt sxnt_sexp0))
-            (seq (rpt (grabWS (pnt sxnt_sexp0))
-                      (FOLDR SX_CONS (SX_SYM "nil")))
-                 (choicel [
-                     pegf (grabWS (tokeq #")")) (K (SX_SYM "nil"));
-                     grabWS (tokeq #".") ~>
-                        grabWS (pnt sxnt_sexp0)
-                     <~ grabWS (tokeq #")")
-                     ])
-                 replace_nil)
-            SX_CONS
-     ]);
-     (mkNT sxnt_WSsexp,
-      rpt (tok isSpace (K arb_sexp)) (K arb_sexp) ~> pnt sxnt_sexp0);
-     (mkNT sxnt_sexpnum,
-        seq (pnt sxnt_digit)
-            (rpt (pnt sxnt_digit)
-                 (UNCURRY SX_CONS o (SX_NUM ## SX_NUM) o
-                  FOLDL (λ(l,n) d. (10*l, 10*n + destSXNUM d)) (1,0)))
-            (λs1. (λ(l,n). SX_NUM (destSXNUM s1 * l + n))
-                  o (destSXNUM ## destSXNUM) o destSXCONS)) ;
-     (mkNT sxnt_digit, tok isDigit (λ(c,l). SX_NUM (ORD c - ORD #"0"))) ;
-     (mkNT sxnt_sexpsym,
-      seq (tok valid_first_symchar (λ(c,l). SX_SYM [c]))
-          (rpt (tok valid_symchar (λ(c,l). SX_SYM [c]))
-               (SX_SYM o FOLDR (λs a. destSXSYM s ++ a) []))
-          (λs1 s2. SX_SYM (destSXSYM s1 ++ destSXSYM s2)));
-     (mkNT sxnt_strcontents,
-      rpt (pnt sxnt_strchar) (SX_STR o FOLDR (λs a. destSXSYM s ++ a) []));
-     (mkNT sxnt_strchar,
-      choicel [
-        tokeq #"\\" ~> pnt sxnt_escapedstrchar ;
-        pnt sxnt_normstrchar
-      ]);
-     (mkNT sxnt_escapedstrchar, choicel [tokeq #"\\"; tokeq #"\""]);
-     (mkNT sxnt_normstrchar,
-      tok (λc. isPrint c ∧ c ≠ #"\"" ∧ c ≠ #"\\") (λ(c,l). SX_SYM [c]))
-    ]
+           [(mkNT sxnt_sexp,
+             pnt sxnt_WSsexp <~ rpt (tok isSpace (K arb_sexp)) (K arb_sexp));
+            (mkNT sxnt_sexp0,
+             choicel [
+                 pnt sxnt_sexpnum ;
+                 tokeq #"(" ~> pnt sxnt_sexpseq ;
+                 tokeq #"\"" ~> pnt sxnt_strcontents <~ tokeq #"\"" ;
+                 pegf (tokeq #"'" ~> grabWS (pnt sxnt_sexp0))
+                      (λs. ⟪ SX_SYM "quote"; s⟫) ;
+                 pnt sxnt_sexpsym
+               ]);
+            (mkNT sxnt_sexpseq,
+             choicel [
+                 pegf (grabWS (tokeq #")")) (K (SX_SYM "nil"));
+                 seq (grabWS (pnt sxnt_sexp0))
+                     (seq (rpt (grabWS (pnt sxnt_sexp0))
+                           (FOLDR SX_CONS (SX_SYM "nil")))
+                      (choicel [
+                          pegf (grabWS (tokeq #")")) (K (SX_SYM "nil"));
+                          grabWS (tokeq #".") ~>
+                                 grabWS (pnt sxnt_sexp0)
+                                 <~ grabWS (tokeq #")")
+                        ])
+                      replace_nil)
+                     SX_CONS
+               ]);
+            (mkNT sxnt_WSsexp,
+             rpt (tok isSpace (K arb_sexp)) (K arb_sexp) ~> pnt sxnt_sexp0);
+            (mkNT sxnt_sexpnum,
+             seq (pnt sxnt_digit)
+                 (rpt (pnt sxnt_digit)
+                  (UNCURRY SX_CONS o (SX_NUM ## SX_NUM) o
+                   FOLDL (λ(l,n) d. (10*l, 10*n + destSXNUM d)) (1,0)))
+                 (λs1. (λ(l,n). SX_NUM (destSXNUM s1 * l + n))
+                       o (destSXNUM ## destSXNUM) o destSXCONS)) ;
+            (mkNT sxnt_digit, tok isDigit (λ(c,l). SX_NUM (ORD c - ORD #"0"))) ;
+            (mkNT sxnt_sexpsym,
+             seq (tok valid_first_symchar (λ(c,l). SX_SYM [c]))
+                 (rpt (tok valid_symchar (λ(c,l). SX_SYM [c]))
+                  (SX_SYM o FOLDR (λs a. destSXSYM s ++ a) []))
+                 (λs1 s2. SX_SYM (destSXSYM s1 ++ destSXSYM s2)));
+            (mkNT sxnt_strcontents,
+             rpt (pnt sxnt_strchar)
+                 (SX_STR o FOLDR (λs a. destSXSYM s ++ a) []));
+            (mkNT sxnt_strchar,
+             choicel [
+                 tokeq #"\\" ~> pnt sxnt_escapedstrchar ;
+                 pnt sxnt_normstrchar
+               ]);
+            (mkNT sxnt_escapedstrchar, choicel [tokeq #"\\"; tokeq #"\""]);
+            (mkNT sxnt_normstrchar,
+             tok (λc. isPrint c ∧ c ≠ #"\"" ∧ c ≠ #"\\") (λ(c,l). SX_SYM [c]))
+           ]
   |>
-`;
+End
 
-val sexpPEG_start = save_thm(
-  "sexpPEG_start[simp]",
-  SIMP_CONV(srw_ss())[sexpPEG_def]``sexpPEG.start``)
-val ds = derive_compset_distincts ``:sexpNT``
-val {lookups,fdom_thm,applieds} = derive_lookup_ths {pegth = sexpPEG_def, ntty = ``:sexpNT``, simp = SIMP_CONV (srw_ss())}
-val sexpPEG_exec_thm = save_thm("sexpPEG_exec_thm",LIST_CONJ(sexpPEG_start::ds::lookups))
-val _ = computeLib.add_persistent_funs["sexpPEG_exec_thm"];
-val _ = save_thm("FDOM_sexpPEG", fdom_thm);
-val _ = save_thm("sexpPEG_applied", LIST_CONJ applieds);
+Theorem sexpPEG_start[simp] = SIMP_CONV(srw_ss())[sexpPEG_def]“sexpPEG.start”
+val ds = derive_compset_distincts “:sexpNT”
+val {lookups,fdom_thm,applieds} =
+  derive_lookup_ths {pegth = sexpPEG_def, ntty = “:sexpNT”,
+                     simp = SIMP_CONV (srw_ss())}
+Theorem sexpPEG_exec_thm[compute] = LIST_CONJ(sexpPEG_start::ds::lookups)
+Theorem FDOM_sexpPEG = fdom_thm
+Theorem sexpPEG_applied = LIST_CONJ applieds
 
-val frange_image = prove(
-  ``FRANGE fm = IMAGE (FAPPLY fm) (FDOM fm)``,
-  simp[finite_mapTheory.FRANGE_DEF, pred_setTheory.EXTENSION] >> metis_tac[]);
+Triviality frange_image:
+  FRANGE fm = IMAGE (FAPPLY fm) (FDOM fm)
+Proof
+  simp[finite_mapTheory.FRANGE_DEF, pred_setTheory.EXTENSION] >> metis_tac[]
+QED
 
-val sexpPEG_range =
+Theorem sexpPEG_range[local] =
     SIMP_CONV (srw_ss())
               (fdom_thm :: frange_image :: applieds)
-              ``FRANGE sexpPEG.rules``
+              “FRANGE sexpPEG.rules”
 
-val wfpeg_rwts = wfpeg_cases
-                   |> ISPEC ``sexpPEG``
-                   |> (fn th => map (fn t => Q.SPEC t th)
-                                    [`seq e1 e2 f`, `choice e1 e2 f`, `tok P f`,
-                                     `any f`, `empty v`, `not e v`, `rpt e f`,
-                                     `choicel []`, `choicel (h::t)`, `tokeq t`,
-                                     `pegf e f`
-                      ])
-                   |> map (CONV_RULE
-                             (RAND_CONV (SIMP_CONV (srw_ss())
-                                [choicel_def, tokeq_def, ignoreL_def,
-                                 ignoreR_def, pegf_def, grabWS_def])))
+val wfpeg_rwts =
+  wfpeg_cases
+    |> ISPEC “sexpPEG”
+    |> (fn th => map (fn t => Q.SPEC t th)
+                     [‘seq e1 e2 f’, ‘choice e1 e2 f’, ‘tok P f’,
+                      ‘any f’, ‘empty v’, ‘not e v’, ‘rpt e f’,
+                      ‘choicel []’, ‘choicel (h::t)’, ‘tokeq t’,
+                      ‘pegf e f’
+       ])
+    |> map (CONV_RULE
+              (RAND_CONV (SIMP_CONV (srw_ss())
+                 [choicel_def, tokeq_def, ignoreL_def,
+                  ignoreR_def, pegf_def, grabWS_def])))
 
 
-val wfpeg_pnt = wfpeg_cases
-                  |> ISPEC ``sexpPEG``
-                  |> Q.SPEC `pnt n`
-                  |> CONV_RULE (RAND_CONV (SIMP_CONV (srw_ss()) [pnt_def]))
+Theorem wfpeg_pnt[local] =
+  wfpeg_cases
+    |> ISPEC “sexpPEG”
+    |> Q.SPEC ‘pnt n’
+    |> CONV_RULE (RAND_CONV (SIMP_CONV (srw_ss()) [pnt_def]))
 
 val peg0_rwts = peg0_cases
-                  |> ISPEC ``sexpPEG`` |> CONJUNCTS
+                  |> ISPEC “sexpPEG” |> CONJUNCTS
                   |> map (fn th => map (fn t => Q.SPEC t th)
-                                       [`tok P f`, `choice e1 e2 f`, `seq e1 e2 f`,
-                                        `tokeq t`, `empty l`, `not e v`, `rpt e f`])
+                                       [‘tok P f’, ‘choice e1 e2 f’,
+                                        ‘seq e1 e2 f’, ‘tokeq t’, ‘empty l’,
+                                        ‘not e v’, ‘rpt e f’])
                   |> List.concat
                   |> map (CONV_RULE
                             (RAND_CONV (SIMP_CONV (srw_ss())
                                                   [tokeq_def])))
 
-val wfpeg_grabWS =
+Theorem wfpeg_grabWS[local] =
   SIMP_CONV (srw_ss()) (grabWS_def::ignoreL_def::wfpeg_rwts @ peg0_rwts)
-                       ``wfpeg sexpPEG (grabWS e)``
+                       “wfpeg sexpPEG (grabWS e)”
 
 
-val pegfail_t = ``pegfail``
+val pegfail_t = “pegfail”
 val peg0_rwts = let
   fun filterthis th = let
     val c = concl th
@@ -183,15 +201,17 @@ in
   List.filter filterthis peg0_rwts
 end
 
-val pegnt_case_ths = peg0_cases
-                      |> ISPEC ``sexpPEG`` |> CONJUNCTS
-                      |> map (Q.SPEC `pnt n`)
-                      |> map (CONV_RULE (RAND_CONV (SIMP_CONV (srw_ss()) [pnt_def])))
+val pegnt_case_ths =
+  peg0_cases
+    |> ISPEC “sexpPEG” |> CONJUNCTS
+    |> map (Q.SPEC ‘pnt n’)
+    |> map (CONV_RULE (RAND_CONV (SIMP_CONV (srw_ss()) [pnt_def])))
 
 fun pegnt(t,acc) = let
   val th =
-      prove(``¬peg0 sexpPEG (pnt ^t)``,
-            simp (fdom_thm::choicel_def::ignoreL_def::ignoreR_def::applieds @ pegnt_case_ths) >>
+      prove(“¬peg0 sexpPEG (pnt ^t)”,
+            simp (fdom_thm::choicel_def::ignoreL_def::ignoreR_def::applieds @
+                  pegnt_case_ths) >>
             simp(peg0_rwts @ acc))
   val nm = "peg0_" ^ term_to_string t
   val th' = save_thm(nm, SIMP_RULE bool_ss [pnt_def] th)
@@ -202,33 +222,38 @@ end
 
 val npeg0_rwts =
     List.foldl pegnt []
-   [``sxnt_symchars``, ``sxnt_symchar``,
-    ``sxnt_strchar``, ``sxnt_sexpsym``, ``sxnt_sexpstr``,
-    ``sxnt_sexpnum``,  ``sxnt_normstrchar``,
-    ``sxnt_grabWS``, ``sxnt_first_symchar``, ``sxnt_escapedstrchar``,
-    ``sxnt_escapablechar``, ``sxnt_digit``,``sxnt_WS``]
+   [“sxnt_symchars”, “sxnt_symchar”,
+    “sxnt_strchar”, “sxnt_sexpsym”, “sxnt_sexpstr”,
+    “sxnt_sexpnum”,  “sxnt_normstrchar”,
+    “sxnt_grabWS”, “sxnt_first_symchar”, “sxnt_escapedstrchar”,
+    “sxnt_escapablechar”, “sxnt_digit”,“sxnt_WS”]
 
-val npeg0_sexp0 = Q.prove(
-  `¬peg0 sexpPEG (pnt sxnt_sexp0)`,
+Theorem npeg0_sexp0[local]:
+  ¬peg0 sexpPEG (pnt sxnt_sexp0)
+Proof
   simp pegnt_case_ths >> simp[fdom_thm] >>
   simp applieds >> simp[ignoreL_def,ignoreR_def] >>
-  simp npeg0_rwts)
+  simp npeg0_rwts
+QED
 
-val npeg0_WSsexp = Q.prove(
-  `¬peg0 sexpPEG (pnt sxnt_WSsexp)`,
+Theorem npeg0_WSsexp[local]:
+  ¬peg0 sexpPEG (pnt sxnt_WSsexp)
+Proof
   simp pegnt_case_ths >> simp[fdom_thm] >>
   simp applieds >> simp[ignoreL_def] >>
-  simp (npeg0_sexp0::peg0_rwts))
+  simp (npeg0_sexp0::peg0_rwts)
+QED
 
 val npeg0_rwts = npeg0_WSsexp::npeg0_sexp0::npeg0_rwts
 
-val peg0_grabWS = Q.prove(
-  `peg0 sexpPEG (grabWS e) = peg0 sexpPEG e`,
-  simp(ignoreL_def::grabWS_def::peg0_rwts));
+Theorem peg0_grabWS[local]:
+  peg0 sexpPEG (grabWS e) = peg0 sexpPEG e
+Proof simp(ignoreL_def::grabWS_def::peg0_rwts)
+QED
 
 fun wfnt(t,acc) = let
   val th =
-    prove(``wfpeg sexpPEG (pnt ^t)``,
+    prove(“wfpeg sexpPEG (pnt ^t)”,
           SIMP_TAC (srw_ss())
                    (applieds @
                     [wfpeg_pnt, fdom_thm, ignoreL_def, ignoreR_def,
@@ -240,27 +265,27 @@ in
 end;
 
 val topo_nts =
-  [``sxnt_sexpsym``,
-   ``sxnt_escapedstrchar``,
-   ``sxnt_normstrchar``,
-   ``sxnt_strchar``,
-   ``sxnt_strcontents``,
-   ``sxnt_digit``,
-   ``sxnt_sexpnum``,
-   ``sxnt_sexp0``,
-   ``sxnt_WSsexp``,
-   ``sxnt_sexpseq``,
-   ``sxnt_sexp``]
+  [“sxnt_sexpsym”,
+   “sxnt_escapedstrchar”,
+   “sxnt_normstrchar”,
+   “sxnt_strchar”,
+   “sxnt_strcontents”,
+   “sxnt_digit”,
+   “sxnt_sexpnum”,
+   “sxnt_sexp0”,
+   “sxnt_WSsexp”,
+   “sxnt_sexpseq”,
+   “sxnt_sexp”]
 
 val wfpeg_thm = LIST_CONJ (List.foldl wfnt [] topo_nts)
 
-val subexprs_pnt = prove(
-  ``subexprs (pnt n) = {pnt n}``,
-  simp[subexprs_def, pnt_def]);
+Theorem subexprs_pnt[local]:
+  subexprs (pnt n) = {pnt n}
+Proof simp[subexprs_def, pnt_def]
+QED
 
-val Gexprs_sexpPEG = save_thm(
-  "Gexprs_sexpPEG",
-  ``Gexprs sexpPEG``
+Theorem Gexprs_sexpPEG =
+  “Gexprs sexpPEG”
     |> SIMP_CONV (srw_ss())
          [Gexprs_def, subexprs_def,
           subexprs_pnt, sexpPEG_start, sexpPEG_range,
@@ -268,13 +293,14 @@ val Gexprs_sexpPEG = save_thm(
           choicel_def, tokeq_def, pegf_def, grabWS_def,
           checkAhead_def,
           pred_setTheory.INSERT_UNION_EQ
-         ])
+         ]
 
-val wfG_sexpPEG = store_thm(
-  "wfG_sexpPEG",
-  ``wfG sexpPEG``,
+Theorem wfG_sexpPEG:
+  wfG sexpPEG
+Proof
   rw[wfG_def,Gexprs_sexpPEG] >>
   srw_tac[boolSimps.DNF_ss][] >>
-  simp(wfpeg_thm :: wfpeg_rwts @ npeg0_rwts));
+  simp(wfpeg_thm :: wfpeg_rwts @ npeg0_rwts)
+QED
 
 val _ = export_theory();
